Fix some errors in blake2f and tweak interface
Progress on #70

util/blake2fScript.sml
@@ -1,5 +1,5 @@
 open HolKernel boolLib bossLib Parse wordsLib cv_transLib
-     cv_stdTheory listTheory wordsTheory
+     cv_stdTheory listTheory wordsTheory byteTheory vfmTypesTheory
 
 val () = new_theory "blake2f";
 
@@ -12,8 +12,8 @@ Definition iv_def:
      0x1F83D9ABFB41BD6Bw; 0x5BE0CD19137E2179w]
 End
 
-EVAL“0x1F83D9ABFB41BD6Bw ⊕
-     0xFFFFFFFFFFFFFFFFw:word32”
+EVAL“0x1F83D9ABFB41BD6Bw ??
+    (0xFFFFFFFFFFFFFFFFw:word64)”
 *)
 
 Definition rotr_def:
@@ -22,8 +22,8 @@ End
 
 val () = cv_auto_trans rotr_def;
 
-Definition g_def:
-  g va vb vc vd x (y:word64) = let
+Definition blake2g_def:
+  blake2g va vb vc vd x (y:word64) = let
     va = va + vb + x;
     vd = rotr 32 (vd ⊕ va);
     vc = vc + vd;
@@ -31,11 +31,11 @@ Definition g_def:
     va = va + vb + y;
     vd = rotr 16 (vd ⊕ va);
     vc = vc + vd;
-    vb = rotr 64 (vb ⊕ vc)
+    vb = rotr 63 (vb ⊕ vc)
   in (va, vb, vc, vd)
 End
 
-val () = cv_auto_trans g_def;
+val () = cv_auto_trans blake2g_def;
 
 Definition sigmas_def:
   sigmas : num list list =
@@ -48,9 +48,7 @@ Definition sigmas_def:
    [12;  5;  1; 15; 14; 13;  4; 10;  0;  7;  6;  3;  9;  2;  8; 11];
    [13; 11;  7; 14; 12;  1;  3;  9;  5;  0; 15;  4;  8;  6;  2; 10];
    [ 6; 15; 14;  9; 11;  3;  0;  8; 12;  2; 13;  7;  1;  4; 10;  5];
-   [10;  2;  8;  4;  7;  6;  1;  5; 15; 11;  9; 14;  3; 12; 13;  0];
-   [ 0;  1;  2;  3;  4;  5;  6;  7;  8;  9; 10; 11; 12; 13; 14; 15];
-   [14; 10;  4;  8;  9; 15; 13;  6;  1; 12;  0;  2; 11;  7;  5;  3]]
+   [10;  2;  8;  4;  7;  6;  1;  5; 15; 11;  9; 14;  3; 12; 13;  0]]
 End
 
 val () = cv_trans_deep_embedding EVAL sigmas_def;
@@ -58,21 +56,21 @@ val () = cv_trans_deep_embedding EVAL sigmas_def;
 Definition body_def:
   body v0 v1 v2 v3 v4 v5 v6 v7 v8 v9 v10 v11 v12 v13 v14 v15 m s = let
     i = HD s; s = TL s; j = HD s; s = TL s;
-    (v0, v4, v8, v12) = g v0 v4 v8 v12 (EL i m) (EL j m);
+    (v0, v4, v8, v12) = blake2g v0 v4 v8 v12 (EL i m) (EL j m);
     i = HD s; s = TL s; j = HD s; s = TL s;
-    (v1, v5, v9, v13) = g v1 v5 v9 v13 (EL i m) (EL j m);
+    (v1, v5, v9, v13) = blake2g v1 v5 v9 v13 (EL i m) (EL j m);
     i = HD s; s = TL s; j = HD s; s = TL s;
-    (v2, v6, v10, v14) = g v2 v6 v10 v14 (EL i m) (EL j m);
+    (v2, v6, v10, v14) = blake2g v2 v6 v10 v14 (EL i m) (EL j m);
     i = HD s; s = TL s; j = HD s; s = TL s;
-    (v3, v7, v11, v15) = g v3 v7 v11 v15 (EL i m) (EL j m);
+    (v3, v7, v11, v15) = blake2g v3 v7 v11 v15 (EL i m) (EL j m);
     i = HD s; s = TL s; j = HD s; s = TL s;
-    (v0, v5, v10, v15) = g v0 v5 v10 v15 (EL i m) (EL j m);
+    (v0, v5, v10, v15) = blake2g v0 v5 v10 v15 (EL i m) (EL j m);
     i = HD s; s = TL s; j = HD s; s = TL s;
-    (v1, v6, v11, v12) = g v1 v6 v11 v12 (EL i m) (EL j m);
+    (v1, v6, v11, v12) = blake2g v1 v6 v11 v12 (EL i m) (EL j m);
     i = HD s; s = TL s; j = HD s; s = TL s;
-    (v2, v7, v8, v13) = g v2 v7 v8 v13 (EL i m) (EL j m);
+    (v2, v7, v8, v13) = blake2g v2 v7 v8 v13 (EL i m) (EL j m);
     i = HD s; s = TL s; j = HD s;
-    (v3, v4, v9, v14) = g v3 v4 v9 v14 (EL i m) (EL j m)
+    (v3, v4, v9, v14) = blake2g v3 v4 v9 v14 (EL i m) (EL j m)
   in
     (v0, v1, v2, v3, v4, v5, v6, v7, v8, v9, v10, v11, v12, v13, v14, v15)
 End
@@ -88,64 +86,75 @@ Proof
 QED
 
 Definition loop_def:
-  loop v0 v1 v2 v3 v4 v5 v6 v7 v8 v9 v10 v11 v12 v13 v14 v15 m [] =
+  loop v0 v1 v2 v3 v4 v5 v6 v7 v8 v9 v10 v11 v12 v13 v14 v15 m ss 0 =
     (v0, v1, v2, v3, v4, v5, v6, v7, v8, v9, v10, v11, v12, v13, v14, v15) ∧
-  loop v0 v1 v2 v3 v4 v5 v6 v7 v8 v9 v10 v11 v12 v13 v14 v15 m (s::ss) =
+  loop v0 v1 v2 v3 v4 v5 v6 v7 v8 v9 v10 v11 v12 v13 v14 v15 m ss (SUC n) =
+  let (s, ss) = case ss of s::ss => (s, ss) | [] => (HD sigmas, TL sigmas) in
   let (v0, v1, v2, v3, v4, v5, v6, v7, v8, v9, v10, v11, v12, v13, v14, v15)
-      = body v0 v1 v2 v3 v4 v5 v6 v7 v8 v9 v10 v11 v12 v13 v14 v15 m s
-  in loop v0 v1 v2 v3 v4 v5 v6 v7 v8 v9 v10 v11 v12 v13 v14 v15 m ss
+   = body v0 v1 v2 v3 v4 v5 v6 v7 v8 v9 v10 v11 v12 v13 v14 v15 m s
+  in loop v0 v1 v2 v3 v4 v5 v6 v7 v8 v9 v10 v11 v12 v13 v14 v15 m ss n
 End
 
 val loop_pre_def = cv_trans_pre loop_def;
 
 Theorem loop_pre_length:
-  EVERY (λs. LENGTH s = 16 ∧ EVERY (λi. i < LENGTH m) s) ss
-  ⇒ loop_pre _ _ _ _ _ _ _ _ _ _ _ _ _ _ _ _ m ss
+  EVERY (λs. LENGTH s = 16 ∧ EVERY (λi. i < LENGTH m) s) (sigmas ++ ss)
+  ⇒ loop_pre _ _ _ _ _ _ _ _ _ _ _ _ _ _ _ _ m ss n
 Proof
   (fn g as (_,w) => map_every ID_SPEC_TAC (free_vars w) g)
-  \\ Induct_on`ss`
+  \\ Induct_on`n`
   \\ rw[Once loop_pre_def]
-  \\ irule body_pre_length \\ rw[]
+  >- rw[sigmas_def]
+  >- (
+    irule body_pre_length
+    \\ gvs[CaseEq"list"]
+    \\ Cases_on`sigmas` >- fs[sigmas_def]
+    \\ gvs[] )
+  \\ gvs[CaseEq"list"]
+  \\ first_x_assum irule
+  \\ Cases_on`sigmas` >- fs[sigmas_def]
+  \\ gvs[]
 QED
 
-Definition f_def:
-  f h0 h1 h2 h3 h4 h5 h6 h7 m t0 t1 (flag: word8) = let
-    v0 = h0;
-    v1 = h1;
-    v2 = h2;
-    v3 = h3;
-    v4 = h4;
-    v5 = h5;
-    v6 = h6;
-    v7 = h7;
+Definition blake2f_def:
+  blake2f r hs m t0 t1 (flag: word8) = let
+    h0 = HD hs; hs = TL hs;
+    h1 = HD hs; hs = TL hs;
+    h2 = HD hs; hs = TL hs;
+    h3 = HD hs; hs = TL hs;
+    h4 = HD hs; hs = TL hs;
+    h5 = HD hs; hs = TL hs;
+    h6 = HD hs; hs = TL hs;
+    h7 = HD hs; hs = TL hs;
     v8 = 0x6A09E667F3BCC908w;
     v9 = 0xBB67AE8584CAA73Bw;
     v10 = 0x3C6EF372FE94F82Bw;
     v11 = 0xA54FF53A5F1D36F1w;
     v12 = 0x510E527FADE682D1w ⊕ t0;
     v13 = 0x9B05688C2B3E6C1Fw ⊕ t1;
-    v14 = if flag = 1w then 0x4BE4294w else 0x1F83D9ABFB41BD6Bw;
+    v14 = if flag = 1w then 0xE07C265404BE4294w else 0x1F83D9ABFB41BD6Bw;
     v15 = 0x5BE0CD19137E2179w;
     (v0, v1, v2, v3, v4, v5, v6, v7, v8, v9, v10, v11, v12, v13, v14, v15)
-    = loop v0 v1 v2 v3 v4 v5 v6 v7 v8 v9 v10 v11 v12 v13 v14 v15 m sigmas;
-    h0 = h0 ?? v0 ?? v8;
-    h1 = h1 ?? v1 ?? v9;
-    h2 = h2 ?? v2 ?? v10;
-    h3 = h3 ?? v3 ?? v11;
-    h4 = h4 ?? v4 ?? v12;
-    h5 = h5 ?? v5 ?? v13;
-    h6 = h6 ?? v6 ?? v14;
-    h7 = h7 ?? v7 ?? v15
-  in (h0, h1, h2, h3, h4, h5, h6, h7)
+    = loop h0 h1 h2 h3 h4 h5 h6 h7 v8 v9 v10 v11 v12 v13 v14 v15 m [] r;
+    h0 = word_to_bytes (h0 ?? v0 ?? v8) F;
+    h1 = word_to_bytes (h1 ?? v1 ?? v9) F;
+    h2 = word_to_bytes (h2 ?? v2 ?? v10) F;
+    h3 = word_to_bytes (h3 ?? v3 ?? v11) F;
+    h4 = word_to_bytes (h4 ?? v4 ?? v12) F;
+    h5 = word_to_bytes (h5 ?? v5 ?? v13) F;
+    h6 = word_to_bytes (h6 ?? v6 ?? v14) F;
+    h7 = word_to_bytes (h7 ?? v7 ?? v15) F;
+  in FLAT [h0;h1;h2;h3;h4;h5;h6;h7]
 End
 
-val f_pre_def = cv_trans_pre f_def;
+val blake2f_pre_def = cv_trans_pre blake2f_def;
 
-Theorem f_pre_length:
-  LENGTH m = 16 ⇒
-  f_pre _ _ _ _ _ _ _ _ m _ _ _
+Theorem blake2f_pre_length:
+  LENGTH hs = 8 ∧ LENGTH m = 16 ⇒
+  blake2f_pre _ hs m _ _ _
 Proof
-  rw[f_pre_def]
+  rw[blake2f_pre_def]
+  \\ gvs[LENGTH_EQ_NUM_compute]
   \\ irule loop_pre_length
   \\ rw[sigmas_def]
 QED
